# 1


# 2


# 3


# 4


# 5

![[Pasted image 20220615005509.png]]

P(n): $1^{2}+ 3^{2}+ 5^{2}+...+ (2n+1)^{2}= \frac{1}{3}(n + 1)(2n + 1)(2n + 3)$

Inductive Step: 
Let k be an arbitrary nonnegative integer

Assume P(k): $1^{2}+ 3^{2}+ 5^{2}+...+ (2k+1)^{2}= \frac{1}{3}(k + 1)(2k + 1)(2k + 3)$

Prove P(k + 1): $1^{2}+2^{2}+3^{2}+...+(2k+1)^{2} + (2k+3)^{2} = \frac{1}{3} (k+2)(2k+3)(2k +5)$
$1^{2}+2^{2}+3^{2}+...+(2k+1)^{2} + (2k+3)^{2}$
$= [\frac{1}{3}(k+1)(2k+1)(2k+3)] + (2k + 3)^2$    By I.H
$= \frac{1}{3} (2k + 3) [(k+1)(2k+1) + 3(2k+3)]$
$= \frac{1}{3} (2k + 3) [2k^2+3k+1+6k+9]$
$=\frac{1}{3}(2k+3)[(2k^{2}+9k+10)]$
$=\frac{1}{3}(2k+3)[(2k+5)(k+2)]$

$=\frac{1}{3}(k+1)(2k+3)(2k+5)$

Hence, if P(k) is true, then P(k + 1) is true. 
This concludes the inductive step. 



By the principle of induction, since the base case and the inductive step are true, we can conclude that $1^2+2^2+3^2+...+(2n+1)^2=\frac{1}{3}(n+1)(2n+1)(2n+3)$ whenever n is a nonnegative integer. 

# 6


# 7


# 8


# 9


# 10


# 11


# 12


# 13


# 14


# 15


# 16


# 17


# 18


# 19


# 20


# 21


# 22


# 23


# 24


# 25


# 26


# 27


# 28


# 29


# 30


# 31


# 32


# 33


# 34


# 35


# 36


# 37


# 38


# 39


# 40


# 41


# 42


# 43


# 44


# 45


# 46


# 47


# 48


# 49


# 50


# 51


# 52


# 53