# ND - Conjunction 

**Links** - [[;1.6 - Natural Deduction]]
[[Conditional]]

---

### What is the $\to$ introduction rule?

![[Pasted image 20220531185103.png]]
This utilizes an assumption box. 
We start it with an assumption, in this case p, and the utilizing the previous lines, we can deduce q. This will allow us to create the statement, p → q. 

This is actually very similar to how proofs in natural deduction are created, where premises → conclusions are like assumptions → conclusions. 

[[Assumption Boxes]]

### What is the $\to$ elimination rule? 

![[Pasted image 20220531185020.png]]

We know that the first statmenet must be true. It could be true if p is false though, so we can’t do much with it. 

But the moment we have that p is true, then we know that q is true. Thus, we can do an conditional elimination, citing both lines. 

